wip

LeanSubst/Basic.lean
@@ -5,78 +5,85 @@ open Lilac
 namespace LeanSubst
 
 universe u1 u2 u3
-variable {S : Type} {T : Type} {U : Type}
+variable {S : Type u1} {T : Type u2} {U : Type u3}
 
-structure Ren (T : Type) : Type where
-  act : Nat -> Nat
+set_option linter.unusedVariables false in
+abbrev Var (T : Type u2) := Nat
 
-class RenMap {n : Nat} (S : Type) (V : Vec (Type) n) where
+structure Ren (T : Type u2) : Type u3 where
+  act : Var T -> Var T
+
+class RenMap {n : Nat} (S : Type u1) (V : Vec (Type u2) n) where
   rmap : V -> S -> S
-  self : Option (V -> Ren S)
+  self [NeZero n] : True ∨ V.head = Ren S
 
 export RenMap (rmap)
 
-macro:max t:term noWs "⟨" r:term "⟩" : term => `(rmap $r $t)
+macro:max (name := «term_⟨_,⟩») t:term noWs "⟨" r:term "," "⟩" : term => `(rmap $r $t)
+syntax:max (name := «term_⟨_,+⟩») term noWs "⟨" term ,+ "⟩" : term
+
+open Lean in
+macro_rules
+  | `($t⟨ $elems,* ⟩) => do
+    let rec expand_ren_lit (i : Nat) (skip : Bool) (result : TSyntax `term) : MacroM Syntax := do
+      match i, skip with
+      | 0,     _     => pure result
+      | i + 1, true  => expand_ren_lit i false result
+      | i + 1, false => expand_ren_lit i true  (<- ``(Tuple.cons $(⟨elems.elemsAndSeps[i]!⟩) $result))
+    let size := elems.elemsAndSeps.size
+    let arg <- expand_ren_lit size (size % 2 == 0) (<- ``(Tuple.nil))
+    let arg : TSyntax `term := .mk arg
+    `(rmap $arg $t)
 
 @[app_unexpander rmap]
 def unexpand_rmap : Lean.PrettyPrinter.Unexpander
 | `($_ $r $t) => `($t⟨$r⟩)
 | _ => throw ()
 
-def test1 : Ren Nat -> Nat -> Nat := sorry
-def test2 : Ren Nat × Ren Bool -> Nat -> Nat := sorry
-
-instance : RenMap Nat #(Ren Nat) where
-  rmap := test1
-  self := sorry
-
-instance : RenMap Nat #(Ren Nat, Ren Bool) where
-  rmap := test2
-  self := sorry
-
-theorem test3 (r1 : Ren Nat) (r2 : Ren Bool) (x : Nat) : x⟨r1::r2::#⟨⟩⟩ = x := sorry
-
-theorem test4 (r1 : Ren Nat) (x : Nat) : x⟨r1::#⟨⟩⟩ = x := sorry
-
-inductive Action (T : Type) where
-| re : Nat -> Action T
+inductive Action (T : Type u2) where
+| re : Var T -> Action T
 | su : T -> Action T
 deriving Repr
 
 export Action (re su)
 
-instance {n} {S : Type} {V : Vec Type n} [i : RenMap S V] : RenMap (Action S) V where
-  self := none
-  rmap := λ r a =>
-    match a with
-    | re x =>
-      match i.self with
-      | some p => re ((p r).act x)
-      | none => re x
-    | su t => su t⟨r⟩
+structure Subst (T : Type u2) where
+  inner : Var T -> Action T
 
--- structure Subst (T : Type u2) where
---   inner : Nat -> Action T
+class SubstAction (T : Type u1) (A : Type u2) (U : outParam (Type u3)) where
+  act (σ : Subst T) : A -> U
 
--- class SubstAction (T : Type u1) (A : Type u2) (U : outParam (Type u3)) where
---   act (σ : Subst T) : A -> U
+def Subst.act [SubstAction S T U] (σ : Subst S) : T -> U := SubstAction.act σ
 
--- def Subst.act [SubstAction S T U] (σ : Subst S) : T -> U := SubstAction.act σ
+instance : SubstAction T Nat (Action T) where
+  act := Subst.inner
 
--- instance : SubstAction T Nat (Action T) where
---   act := Subst.inner
+class SubstMap {n} (S : Type u2) (V : Vec (Type u2) n) where
+  smap : V -> S -> S
+  index : Fin n
+  index_eq : (V[index]) = (Subst S)
 
--- class SubstMap {n} (S : Type u1) (V : Vec (Type u2) n) where
---   smap : V.map Subst -> S -> S
+export SubstMap (smap)
 
--- export SubstMap (smap)
+macro:max (name := «term_[_,]») t:term noWs "[" σ:term "," "]" : term => `(smap $σ $t)
+syntax:max (name := «term_[_,+]») term noWs "[" term ,+ "]" : term
 
--- macro:max t:term noWs "[" σ:term "]" : term => `(smap $σ $t)
+open Lean in
+macro_rules
+  | `($t[ $elems,* ]) => do
+    let rec expand_subst_lit (i : Nat) (skip : Bool) (result : TSyntax `term) : MacroM Syntax := do
+      match i, skip with
+      | 0,     _     => pure result
+      | i + 1, true  => expand_subst_lit i false result
+      | i + 1, false => expand_subst_lit i true  (<- ``(Tuple.cons $(⟨elems.elemsAndSeps[i]!⟩) $result))
+    let size := elems.elemsAndSeps.size
+    let arg <- expand_subst_lit size (size % 2 == 0) (<- ``(Tuple.nil))
+    let arg : TSyntax `term := .mk arg
+    `(smap $arg $t)
 
--- @[app_unexpander smap]
--- def unexpand_smap : Lean.PrettyPrinter.Unexpander
--- | `($_ $σ $t) => `($t[$σ])
--- | _ => throw ()
-
+@[app_unexpander smap]
+def unexpand_smap : Lean.PrettyPrinter.Unexpander
+| `($_ $σ $t) => `($t[$σ])
+| _ => throw ()
 
 end LeanSubst
